pico-ifc-coq/dyn_allocation/RefinementAC.v
@@ -37,6 +37,10 @@ Context {T: Type}
         {CLatt: ConcreteLattice T}
         {WFCLatt: WfConcreteLattice cblock T Latt CLatt}.
 
+Variable t1 : ASysTable T T.
+Variable t2 : ASysTable T unit.
+Hypothesis Ht1t2 : match_asystables t1 t2.
+
 Definition tini_fetch_rule_withsig :=
   (fun opcode => existT _
                         (QuasiAbstractMachine.labelCount opcode)
@@ -47,10 +51,10 @@ Definition tini_match_states := match_states cblock QuasiAbstractMachine.fetch_r
 Definition tini_concrete_machine := concrete_machine cblock tini_faultHandler.
 
 Program Definition abstract_concrete_ref :
-  refinement abstract_machine tini_concrete_machine :=
+  refinement (abstract_machine t1) tini_concrete_machine :=
   @ref_composition _ _ _
-                   abstract_quasi_abstract_ref
-                   (quasi_abstract_concrete_ref stamp_cblock fetch_rule)
+                   (abstract_quasi_abstract_ref Ht1t2)
+                   (quasi_abstract_concrete_ref stamp_cblock fetch_rule t2)
                    (@ac_match_initial_data _ _ _ _ fetch_rule)
                    match_events
                    _ _.
